

# Transition to Theoretical Mathematics

Proof Portfolio

*Shukry Zablah*

*18 December, 2018*

## Contents

|   |          |
|---|----------|
| <b>1 Proof By Cases (Triangle Inequality)</b> | <b>1</b> |
| <b>2 Set Proof</b>                            | <b>3</b> |
| <b>3 Direct Proof</b>                         | <b>4</b> |
| <b>4 Contradiction Proof</b>                  | <b>5</b> |
| <b>5 Contraposition Proof</b>                 | <b>6</b> |
| <b>6 Induction Proof</b>                      | <b>7</b> |

## 1 Proof By Cases (Triangle Inequality)

**Theorem 1** (The Triangle Inequality). *For each pair of real numbers  $x$  and  $y$ , one has that:*

$$|x + y| \leq |x| + |y|.$$

(Hint: Consider cases like  $x, y \geq 0$  or  $x, y \leq 0$  or  $x \geq 0$  and  $y < 0$ , etc.. These cases will help you evaluate the absolute value using its definition.)

*Proof.* We proceed by cases.

**Case 1:**  $x \geq 0$  and  $y \geq 0$ .

Note that by the definition of absolute value and since  $x \geq 0$  and  $y \geq 0$ , we have that  $|x| = x$  and  $|y| = y$  and  $|x + y| = x + y$  (since  $x + y \geq 0$ ).

Thus it follows that  $|x + y| \leq |x| + |y|$  (since  $|x + y| = |x| + |y|$ ).

**Case 2:**  $x < 0$  and  $y < 0$ .

Note that by the definition of absolute value and since  $x < 0$  and  $y < 0$ , we have that  $|x| = -x$  and  $|y| = -y$  and  $|x + y| = -(x + y) = -x - y$  (since  $x + y < 0$ ).

Thus it follows that  $|x + y| \leq |x| + |y|$  (since  $|x + y| = |x| + |y|$ ).

**Case 3:**  $x \geq 0$  and  $y < 0$ .

Note that by the definition of absolute value and since  $x \geq 0$  and  $y < 0$ , we have that  $|x| = x$  and  $|y| = -y$ . Now we need to consider two subcases in which  $|x + y|$  can satisfy  $|x + y| \geq 0$  or  $|x + y| < 0$ .

Suppose that  $|x + y| \geq 0$ . By the definition of absolute value it follows that  $|x + y| = x + y$ . Note that  $x - y \geq x + y$  because  $y$  is negative. By substituting we get that  $|x + y| \leq |x| + |y|$ .

Now suppose that  $|x + y| < 0$ . Observe that  $|x + y| \leq x$ . Since  $y$  is negative we have that  $|x + y| < x - y$ . After substituting equivalent values we have that  $|x + y| \leq |x| + |y|$ .

Since in Case 3 we have that  $x$  and  $y$  are arbitrary, we have exhausted the cases and we have that  $|x + y| \leq |x| + |y|$  for all  $\mathbb{R}$ .

■

## 2 Set Proof

Let  $f : A \rightarrow B$  be a function. Prove the following statements.

**Claim 1.** Let  $C, D \subseteq B$ . Then  $f^{-1}(C) \cup f^{-1}(D) = f^{-1}(C \cup D)$ .

*Proof.* We will show that Claim 1 is true by showing  $f^{-1}(C) \cup f^{-1}(D) \subseteq f^{-1}(C \cup D)$  and  $f^{-1}(C \cup D) \subseteq f^{-1}(C) \cup f^{-1}(D)$ .

We first show that  $f^{-1}(C) \cup f^{-1}(D) \subseteq f^{-1}(C \cup D)$ . By definition of a subset, given an arbitrary element  $x$ , the statement we are trying to show is equivalent to the statement that if  $x \in f^{-1}(C) \cup f^{-1}(D)$  then  $x \in f^{-1}(C \cup D)$ .

Let us assume that  $x \in f^{-1}(C) \cup f^{-1}(D)$ . We assume that it is the case that  $x \in f^{-1}(C)$  then by definition of the preimage we know that  $f(x) \in C$ . Logically, it would also be true that  $f(x) \in C \cup f(x) \in D$ . Then observe that since  $f(x) \in (C \cup D)$ , again, by the definition of preimage it follows that  $x \in f^{-1}(C \cup D)$ . The argument for the case in which  $x \in f^{-1}(D)$  follows the same argument. Therefore, we have that  $f^{-1}(C) \cup f^{-1}(D) \subseteq f^{-1}(C \cup D)$  as desired.

Now, we proceed to show that  $f^{-1}(C \cup D) \subseteq f^{-1}(C) \cup f^{-1}(D)$ . Given an element  $x$ , assume that  $x \in f^{-1}(C \cup D)$ . We will show that  $x \in f^{-1}(C) \cup f^{-1}(D)$ .

By the definition of preimage we have that  $f(x) \in (C \cup D)$ . However, if  $f(x)$  is in the union of  $C$  and  $D$  then logically it follows that  $f(x) \in C \cup f(x) \in D$ . By the definition of preimage it holds true that  $x \in f^{-1}(C) \cup f^{-1}(D)$ . Therefore it is true that  $f^{-1}(C \cup D) \subseteq f^{-1}(C) \cup f^{-1}(D)$ .

Since we have shown that  $f^{-1}(C) \cup f^{-1}(D) \subseteq f^{-1}(C \cup D)$  is true and that  $f^{-1}(C \cup D) \subseteq f^{-1}(C) \cup f^{-1}(D)$  is also true, then by definition we have that  $f^{-1}(C) \cup f^{-1}(D) = f^{-1}(C \cup D)$  as desired. ■

**Claim 2.** Let  $C, D \subseteq A$ . If  $f$  is injective then  $f(C) \cap f(D) \subseteq f(C \cap D)$ .

*Proof.* ■

### 3 Direct Proof

**Claim 1.**  $\lim_{n \rightarrow \infty} \frac{3n}{n+2} = 3$

*Proof.* To show Claim1 we will first fix  $\varepsilon \in (0, \infty)$  arbitrary. Then, we define  $N := \lceil 6/\varepsilon \rceil + 1 \in \mathbb{N}$ . Now we fix  $n \in \mathbb{N}$ , arbitrary and assume that  $n \geq \lceil 6/\varepsilon \rceil + 1$ .

Observe that from the previous statement it follows that  $n \geq 6/\varepsilon + 1$  and  $n > 6/\varepsilon$ . We can also write that  $\varepsilon > 6/n$ . Observe that  $\varepsilon > \frac{6}{n+2}$ . We can rewrite the equivalent statement  $\left| \frac{3n}{n+2} - \frac{3n+6}{n+2} \right|$  and from this we have that  $\left| \frac{3n}{n+2} - 3 \right| < \varepsilon$ .

Since we had fixed  $n$  and  $\varepsilon$  arbitrary, then by the definition of a convergent sequence it follows that  $\lim_{n \rightarrow \infty} \frac{3n}{n+2} = 3$  as desired.

■

## 4 Contradiction Proof

Let  $\prod_{n=1}^{\infty} \mathbb{N} := \mathbb{N} \times \mathbb{N} \times \cdots \times \mathbb{N} \times \cdots := \{(a_1, a_2, \dots, a_n, \dots) : a_n \in \mathbb{N}, \forall n \in \mathbb{N}\}$ .

**Claim 1.**  $\prod_{n=1}^{\infty} \mathbb{N}$  is uncountable.

*Proof.* We proceed to show the original statement is true by contradiction.

Assume to the contrary that  $\prod_{n=1}^{\infty} \mathbb{N}$  is countable. By definition it follows that there exists a bijection

$\varphi : \mathbb{N} \rightarrow \prod_{n=1}^{\infty} \mathbb{N}$ . Seeking a contradiction, we will show how  $\varphi$  cannot be surjective.

Since  $\varphi$  is bijective, we know that  $f(n) \in \prod_{n=1}^{\infty} \mathbb{N}$  for every  $n \in \mathbb{N}$ . For every  $n \in \mathbb{N}$  we can write  $f(n) = (a_1^{(n)}, a_2^{(n)}, a_3^{(n)}, \dots, a_m^{(n)}, \dots)$ , where  $m \in \mathbb{N}$ .

Let's define  $x \in \prod_{n=1}^{\infty} \mathbb{N}$  by setting  $a_m^{(n)} := \begin{cases} 3 & \text{if } a_n^{(n)} \neq 3 \\ 4 & \text{if } a_n^{(n)} = 3 \end{cases}$  for every  $k \in \mathbb{N}$ .

Thus, by construction we have that  $x \neq f(n)$  for every  $n \in \mathbb{N}$  since  $a_m^{(n)} \neq a_n^{(n)}$ .

At this point we have that  $x \in \prod_{n=1}^{\infty} \mathbb{N}$  but also for every  $n \in \mathbb{N}$  we have that  $x \notin f(n)$ . This means that by definition,  $\varphi$  cannot be surjective, and since  $\varphi$  had been said to be bijective, is a contradiction.

Hence, we have that shown that the original statement that  $\prod_{n=1}^{\infty} \mathbb{N}$  is uncountable is true. ■

## 5 Contraposition Proof

## 6 Induction Proof

Proof the following claims.

**Claim 1.** Show that  $2^n \leq 3^n$  for each  $n \in \mathbb{N}$ .

*Proof.* We proceed to prove the statement by induction.

Let us consider the base case when  $n = 1$ . Observe that we have that  $2^1 \leq 3^1$  which is true.

Now we have to show that for every  $n \in \mathbb{N}$  it follows that if  $2^n \leq 3^n$  then  $2^{n+1} \leq 3^{n+1}$ .

We now fix  $n$  arbitrary and assume that  $2^n \leq 3^n$ .

It follows from the inductive hypothesis that  $2 * 2^n \leq 2 * 3^n$ . Observe that since  $2 < 3$  we have that  $2 * 2^n \leq 2 * 3^n \leq 3 * 3^n$ .

Thus it follows that  $2^{n+1} \leq 3^{n+1}$ . Since  $n$  was fixed arbitrary, the same holds for every  $n \in \mathbb{N}$ .

By the Principle of Mathematical Induction we conclude Claim 1 as desired. ■

**Claim 2.**

Use Claim 1 to prove that  $2^n + 1 \leq 3^n$  for every  $n \in \mathbb{N}$ .

*Proof.* We will show that Claim 2 is true by induction.

Consider our base case when  $n = 1$ . Note that  $2^1 + 1 \leq 3^1$  is true.

In our inductive step we now show that for every  $n \in \mathbb{N}$  we have that if  $2^n + 1 \leq 3^n$  then  $2^{n+1} + 1 \leq 3^{n+1}$ .

Fix  $n$  arbitrary. We assume  $2^n + 1 \leq 3^n$ . From the inductive hypothesis it follows that  $2 * (2^n + 1) \leq 3 * (3^n)$  because  $2 < 3$ . Then, it is true that  $2^{n+1} + 2 \leq 3^{n+1}$ . By rearranging the terms we get that  $2 \leq 3^{n+1} - 2^{n+1}$ . At this point observe that  $1 < 2$ , which means that  $1 \leq 3^{n+1} - 2^{n+1}$ . After rearranging the terms again we now get that  $2^{n+1} + 1 \leq 3^{n+1}$ . Recall that  $n$  was fixed arbitrary, which means that we have shown the inductive step is true as desired.

Thus, we have shown Claim 2 is true by the Principle of Mathematical Induction. ■

**Claim 3.**

Is it true that  $2^n + n \leq 3^n$  for every  $n \in \mathbb{N}$ ?

*Proof.* Proceeding by induction, we consider the base case when  $n = 1$ . We know that  $2^1 + 1 \leq 3^1 = 3 \leq 3$ .

Focusing now on the inductive step, we have to show that for every  $n \in \mathbb{N}$  it follows that if  $2^n + n \leq 3^n$  then it is also true that  $2^{n+1} + (n+1) \leq 3^{n+1}$ .

After fixing  $n$  arbitrary, assume that  $2^n + n \leq 3^n$ . In a similar vein as in the previous proof, we use the fact that  $2 < 3$  and our inductive hypothesis to get that  $2 * (2^n + n) \leq 3 * (3^n)$ . After simplifying and rearranging the terms we have that  $2n \leq 3^{n+1} - 2^{n+1}$ . Seeking to show the inductive step we use the fact that  $1 \leq n$  for every  $n \in \mathbb{N}$  to deduce that for every  $n \in \mathbb{N}$  we have that  $n + 1 \leq 2n$ . Using this fact, we can now rewrite our argument as  $n + 1 \leq 3^{n+1} - 2^{n+1}$ . Finally, after rearranging the terms we can see that  $2^{n+1} + (n+1) \leq 3^{n+1}$ . Since  $n$  was fixed arbitrary, we know that the same statement holds true for every  $n \in \mathbb{N}$  as desired.

By the Principle of Mathematical Induction it follows that  $2^n + n \leq 3^n$  for every  $n \in \mathbb{N}$ . ■